Code restructuring.
* Move PrimaryForView to ClusterConfig.
* Move functionality from checked that is not related to
  signature checks to valid predicate.
* Remove LiteInv from replicas and move it into the global Inv
  but renamed to RecordedNewViewMsgsAreValid.

docs/sbft-formal-model/cluster_config.s.dfy
@@ -14,6 +14,8 @@ include "network.s.dfy"
 module ClusterConfig {
   import opened HostIdentifiers
 
+  type ViewNum = nat
+
   datatype Constants = Constants(
     maxByzantineFaultyReplicas:nat,
     numClients:nat,
@@ -30,6 +32,12 @@ module ClusterConfig {
       requires WF()
     {
       N() + numClients
+    }
+
+    function PrimaryForView(view:ViewNum) : nat 
+      requires WF()
+    {
+      view % N()
     }
 
     function F() : nat
