docs/sbft-formal-model/messages.dfy
@@ -17,10 +17,9 @@ module Messages {
   import Library
   import opened HostIdentifiers
   import Network
-  import ClusterConfig
+  import opened ClusterConfig
 
   type SequenceID = nat
-  type ViewNum = nat
 
   datatype ClientOperation = ClientOperation(sender:HostId, timestamp:nat)
 
@@ -56,13 +55,15 @@ module Messages {
   }
 
   datatype ViewChangeMsgsSelectedByPrimary = ViewChangeMsgsSelectedByPrimary(msgs:set<Network.Message<Message>>) {
-    predicate valid(view:ViewNum, quorumSize:nat) {
+    predicate valid(view:ViewNum, clusterConfig:ClusterConfig.Constants) 
+      requires clusterConfig.WF()
+    {
       && |msgs| > 0
       && (forall v | v in msgs :: && v.payload.ViewChangeMsg?
-                                  && v.payload.validViewChangeMsg(quorumSize)
+                                  && v.payload.validViewChangeMsg(clusterConfig)
                                   && v.payload.newView == view) // All the ViewChange messages have to be for the same View. 
       && UniqueSenders(msgs)
-      && |msgs| == quorumSize //TODO: once proof is complete try with >=
+      && |msgs| == clusterConfig.AgreementQuorum() //TODO: once proof is complete try with >=
     }
   }
 
@@ -104,10 +105,11 @@ module Messages {
                      | NewViewMsg(newView:ViewNum, vcMsgs:ViewChangeMsgsSelectedByPrimary) 
                      | CheckpointMsg(seqIDReached:SequenceID, committedClientOperations:CommittedClientOperations)
                      {
-                       predicate valid(quorumSize:nat)
+                       predicate valid(clusterConfig:ClusterConfig.Constants)
+                         requires clusterConfig.WF()
                        {
-                         && (ViewChangeMsg? ==> validViewChangeMsg(quorumSize))
-                         && (NewViewMsg? ==> validNewViewMsg(quorumSize))
+                         && (ViewChangeMsg? ==> validViewChangeMsg(clusterConfig))
+                         && (NewViewMsg? ==> validNewViewMsg(clusterConfig))
                        }
                        predicate checked(clusterConfig:ClusterConfig.Constants, sigChecks:set<Network.Message<Message>>)
                          requires clusterConfig.WF()
@@ -115,36 +117,39 @@ module Messages {
                          && (ViewChangeMsg? ==> checkedViewChangeMsg(clusterConfig, sigChecks))
                          && (NewViewMsg? ==> checkedNewViewMsg(clusterConfig, sigChecks))
                        }
-                       predicate validViewChangeMsg(quorumSize:nat) 
+                       predicate validViewChangeMsg(clusterConfig:ClusterConfig.Constants)
+                         requires clusterConfig.WF()
                          requires ViewChangeMsg?
                        {
-                         proofForLastStable.valid(lastStableCheckpoint, quorumSize)
+                         && (forall seqID | seqID in certificates
+                                  :: && (forall replica | replica in sendersOf(certificates[seqID].votes)
+                                                      :: clusterConfig.IsReplica(replica))
+                                     && certificates[seqID].valid(clusterConfig.AgreementQuorum(), seqID))
+                         && proofForLastStable.valid(lastStableCheckpoint, clusterConfig.AgreementQuorum())
                        }
-                       predicate validNewViewMsg(quorumSize:nat) 
+                       predicate validNewViewMsg(clusterConfig:ClusterConfig.Constants)
+                         requires clusterConfig.WF()
                          requires NewViewMsg?
                        {
-                         vcMsgs.valid(newView, quorumSize)
+                         && vcMsgs.valid(newView, clusterConfig)
+                         && (forall replica | replica in sendersOf(vcMsgs.msgs)
+                                              :: clusterConfig.IsReplica(replica))
                        }
                        predicate checkedViewChangeMsg(clusterConfig:ClusterConfig.Constants, sigChecks:set<Network.Message<Message>>)
                          requires ViewChangeMsg?
                          requires clusterConfig.WF()
                        {
-                          && valid(clusterConfig.AgreementQuorum())
+                          && valid(clusterConfig)
                           // Check Checkpoint msg-s signatures:
                           && proofForLastStable.msgs <= sigChecks
                           && (forall seqID | seqID in certificates
-                                  :: && certificates[seqID].votes <= sigChecks
-                                     && (forall replica | replica in sendersOf(certificates[seqID].votes)
-                                                      :: clusterConfig.IsReplica(replica))
-                                     && certificates[seqID].valid(clusterConfig.AgreementQuorum(), seqID))
+                                  :: && certificates[seqID].votes <= sigChecks)
                        }
                        predicate checkedNewViewMsg(clusterConfig:ClusterConfig.Constants, sigChecks:set<Network.Message<Message>>)
                          requires NewViewMsg?
                          requires clusterConfig.WF()
                        {
-                          && valid(clusterConfig.AgreementQuorum())
-                          && (forall replica | replica in sendersOf(vcMsgs.msgs)
-                                               :: clusterConfig.IsReplica(replica))
+                          && valid(clusterConfig)
                           && vcMsgs.msgs <= sigChecks
                        }
                        predicate IsIntraViewMsg() {
